concurrency/hack-hash-table/MapSpec.s.dfy
@@ -22,10 +22,12 @@ module MapIfc refines InputOutputIfc {
   datatype Input =
     | QueryInput(key: Key)
     | InsertInput(key: Key, value: Value)
+    | RemoveInput(key: Key)
 
   datatype Output =
     | QueryOutput(res: QueryResult)
     | InsertOutput
+    | RemoveOutput
 }
 
 module AsyncIfc {
@@ -61,6 +63,9 @@ module MapSpec {
           case InsertInput(key, value) =>
             && s'.m == s.m[key := value]
             && output == Ifc.InsertOutput
+          case RemoveInput(key) =>
+            && s'.m == s.m - {key}
+            && output == Ifc.RemoveOutput
         }
       )
     }
